1) Vminus does not work with ott 21.2 and the new dominance analysis    interface. In the release, we use ott 20.1 to compile Vminus with the    old dominance interface. kildall.v and lattice.v were copied from    vol/src that use old interfaces. 2) simplified some lemmas in Vminus to match the writing. 3) added Transforms/README to define the mapping between Coq code and    writing. 4) added Transforms/README-popl13 as the top-level readme 5) added Vellvm/Dominators/READ<E-cpp12 for the CPP12 release 6) added release.sh as a script for release 7) We released the revison on our website, and also removed some    irrevelant "Require" from the code.
git-svn-id: https://webdav.seas.upenn.edu/svn/sol/vol@4163 eef5ea85-cc2e-0410-bd84-0fae1f012da8

src3.0/Transforms/vmem2reg_opt_correct.v
@@ -2574,6 +2574,472 @@ Proof.
       destruct (id_dec id0 id0); simpl in Hnst1; try congruence.   
 Qed.
 
+Definition alloca_in_cmd (id':id) (c:cmd) : bool :=
+match c with
+| insn_alloca qid _ _ _ => id_dec id' qid
+| _ => false
+end.
+
+Definition alloca_in_cmds (id':id) (cs:cmds) : bool :=
+(List.fold_left (fun re c => re || alloca_in_cmd id' c) cs false).
+
+Lemma alloca_in_cmds_merge: forall i0 cs1 cs2,
+  alloca_in_cmds i0 cs1 = false /\ alloca_in_cmds i0 cs2 = false ->
+  alloca_in_cmds i0 (cs1++cs2) = false.
+Proof.
+  unfold alloca_in_cmds.
+  intros.
+  rewrite fold_left_app.
+  destruct H as [H1 H2].
+  rewrite H1. auto.
+Qed.
+
+Lemma find_next_stld_inr_intro: forall c0 cs01 pid cs02
+  (Hnst : store_in_cmds pid cs01 = false)
+  (Hst : store_in_cmd pid c0 = true) (Hnld : load_in_cmds pid cs01 = false),
+  exists v1 : value,
+    ret inr (getCmdLoc c0, v1) = find_next_stld (cs01 ++ c0 :: cs02) pid.
+Proof.
+  intros.
+  rewrite <- find_next_stld_strengthen; auto.
+  destruct c0; tinv Hst.
+  destruct value2; tinv Hst.
+  simpl in Hst. simpl.
+  destruct (id_dec id0 pid); subst; tinv Hst.
+  destruct_if; eauto.
+    congruence.
+Qed.
+
+Lemma find_next_stld_inl_intro: forall c0 cs01 pid cs02
+  (Hnst : store_in_cmds pid cs01 = false)
+  (Hld : load_in_cmd pid c0 = true) (Hnld : load_in_cmds pid cs01 = false),
+  ret inl (getCmdLoc c0) = find_next_stld (cs01 ++ c0 :: cs02) pid.
+Proof.
+  intros.
+  rewrite <- find_next_stld_strengthen; auto.
+  destruct c0; tinv Hld.
+  destruct value1; tinv Hld.
+  simpl in Hld. simpl.
+  destruct (id_dec id0 pid); subst; tinv Hld.
+  destruct_if; eauto.
+    congruence.
+Qed.
+
+(***************************************************************)
+
+Module TEST.
+
+Definition wf_cs_action (cs:cmds) (pid:id) (elt:id * action): Prop :=
+let '(id', ac') := elt in
+match ac' with
+| AC_remove =>  
+    exists v0, exists cs0, exists id1, exists v1, exists dones,
+      Some (inl (id', v0, cs0)) = find_init_stld cs pid dones /\
+      Some (inr (id1, v1)) = find_next_stld cs0 pid
+| AC_vsubst v' =>  
+    exists id0, exists cs0, exists dones,
+      Some (inl (id0, v', cs0)) = find_init_stld cs pid dones /\
+      Some (inl id') = find_next_stld cs0 pid
+| AC_tsubst t' =>
+    exists cs0, exists dones,
+      Some (inr (value_const (const_undef t'), cs0)) = 
+        find_init_stld cs pid dones /\
+      Some (inl id') = find_next_stld cs0 pid
+end.
+
+Definition loads_must_be_in_pre (acs: AssocList action) (pid:id) (cs:cmds)
+  : Prop :=
+Forall (fun c => load_in_cmd pid c = true -> getCmdLoc c `in` dom acs) cs.
+
+Definition wf_cs_action_pre (acs: AssocList action) (cs:cmds) (pid:id) 
+  (elt:id * action): Prop :=
+let '(id', ac') := elt in
+match ac' with
+| AC_remove =>  
+    exists v0, exists cs01, exists c0, exists cs02, exists dones,    
+      Some (inl (id', v0, cs01 ++ c0 :: cs02)) = find_init_stld cs pid dones /\
+      store_in_cmds pid cs01 = false /\
+      store_in_cmd pid c0 = true /\ loads_must_be_in_pre acs pid cs01
+| AC_vsubst v' =>  
+    exists id0, exists cs01, exists c0, exists cs02, exists dones,    
+      Some (inl (id0, v', cs01 ++ c0 :: cs02)) = find_init_stld cs pid dones /\
+      store_in_cmds pid cs01 = false /\ getCmdLoc c0 = id' /\
+      load_in_cmd pid c0 = true /\ loads_must_be_in_pre acs pid cs01
+| AC_tsubst t' =>
+    exists cs01, exists c0, exists cs02, exists dones,
+      Some (inr (value_const (const_undef t'), cs01 ++ c0 :: cs02)) = 
+        find_init_stld cs pid dones /\
+      store_in_cmds pid cs01 = false /\ getCmdLoc c0 = id' /\
+      load_in_cmd pid c0 = true /\ loads_must_be_in_pre acs pid cs01
+end.
+
+Lemma loads_must_be_in_nil__no_loads: forall pid cs 
+  (H: loads_must_be_in_pre nil pid cs), load_in_cmds pid cs = false.
+Proof.
+  induction 1; simpl; auto.
+    apply load_in_cmds_false_cons_intro; auto.
+      case_eq (load_in_cmd pid x); auto.
+        intro Heq.
+        apply H in Heq. fsetdec.
+Qed.
+
+Lemma wf_cs_action_nil__wf_cs_action: forall cs pid elt
+  (Hwf: wf_cs_action_pre nil cs pid elt), wf_cs_action cs pid elt.
+Proof.
+  unfold wf_cs_action_pre, wf_cs_action.
+  destruct elt as [id' [|v'|t']]; simpl; intros.
+  Case "1".
+    destruct Hwf as [v0 [cs01 [c0 [cs02 [dones [Hfind1 [Hnst [Hst Hnld]]]]]]]].
+    exists v0. exists (cs01 ++ c0 :: cs02). exists (getCmdLoc c0).
+    apply loads_must_be_in_nil__no_loads in Hnld.    
+    eapply find_next_stld_inr_intro with (cs02:=cs02) in Hnld; eauto.
+    destruct Hnld as [v1 Hnld]. eauto.
+  Case "2".
+    destruct Hwf 
+      as [id0 [cs01 [c0 [cs02 [dones [Hfind1 [Hnst [Heq [Hld Hnld]]]]]]]]]; subst.
+    exists id0. exists (cs01 ++ c0 :: cs02). exists dones.
+    apply loads_must_be_in_nil__no_loads in Hnld.    
+    eapply find_next_stld_inl_intro with (cs02:=cs02) in Hnld; eauto.
+  Case "3".
+    destruct Hwf 
+      as [cs01 [c0 [cs02 [dones [Hfind1 [Hnst [Heq [Hld Hnld]]]]]]]]; subst.
+    exists (cs01 ++ c0 :: cs02). exists dones.
+    apply loads_must_be_in_nil__no_loads in Hnld.    
+    eapply find_next_stld_inl_intro with (cs02:=cs02) in Hnld; eauto.
+Qed.
+
+Definition wf_stld_state (cs:cmds) (pid:id) (elt :stld_state * AssocList action)
+  : Prop :=
+let '(s, acs) := elt in
+match s with
+| STLD_init => alloca_in_cmds pid cs = false /\ store_in_cmds pid cs = false
+| STLD_store id0 v0 =>
+    exists cs1 : list cmd, exists ty0 : typ, exists al0 : align, exists cs2, 
+      cs = cs1 ++ insn_store id0 ty0 v0 (value_id pid) al0 :: cs2 /\
+      store_in_cmds pid cs2 = false /\ loads_must_be_in_pre acs pid cs2
+| STLD_alloca t0 =>
+    exists cs1, exists num, exists al, exists cs2, 
+      cs = cs1 ++ insn_alloca pid t0 num al :: cs2 /\
+      store_in_cmds pid cs2 = false /\ loads_must_be_in_pre acs pid cs2
+end.
+
+Lemma loads_must_be_in_pre_append: forall acs pid cs3 c
+  (Hlds: loads_must_be_in_pre acs pid cs3) (Hld: load_in_cmd pid c = false),
+  loads_must_be_in_pre acs pid (cs3 ++ [c]).
+Proof.
+  intros.
+  apply Forall_forall.
+  intros x Hinx H.
+  destruct_in Hinx.
+    eapply Forall_forall in Hlds; eauto.
+    destruct_in Hinx. congruence.
+Qed.
+
+Lemma wf_stld_state_append: forall st cs1 pid c 
+  (Hwf: wf_stld_state cs1 pid st)
+  (Hnot: alloca_in_cmd pid c = false /\ 
+         store_in_cmd pid c = false /\ 
+         load_in_cmd pid c = false),
+  wf_stld_state (cs1 ++ [c]) pid st.
+Proof.
+  intros.
+  destruct st as [s acs].
+  destruct Hnot as [J1 [J2 J3]].
+  destruct s; simpl in *.
+    destruct Hwf.
+    split.
+      apply alloca_in_cmds_merge; auto.
+      apply store_in_cmds_merge; auto.
+
+    destruct Hwf as [cs2 [t0 [al0 [cs3 [EQ [G1 G2]]]]]]; subst.
+    exists cs2. exists t0. exists al0. exists (cs3 ++ [c]).
+    simpl_env.
+    split; auto.
+    split.
+      apply store_in_cmds_merge; auto.
+      apply loads_must_be_in_pre_append; auto.
+
+    destruct Hwf as [cs2 [num0 [al0 [cs3 [EQ [G1 G2]]]]]]; subst.
+    exists cs2. exists num0. exists al0. exists (cs3 ++ [c]).
+    simpl_env.
+    split; auto.
+    split.
+      apply store_in_cmds_merge; auto.
+      apply loads_must_be_in_pre_append; auto.
+Qed.
+
+Lemma loads_must_be_in_pre_weaken: forall acs1 acs2 pid cs 
+  (Hlds: loads_must_be_in_pre acs2 pid cs),
+  loads_must_be_in_pre (acs1++acs2) pid cs.
+Proof.
+  induction 1; constructor; auto.
+    intro Heq. apply H in Heq. rewrite dom_app. auto.
+Qed.
+
+Lemma loads_must_be_in_pre_append': forall ac acs pid cs3 c
+  (Hlds: loads_must_be_in_pre acs pid cs3) (Hld: load_in_cmd pid c = true)
+  (Heq: fst ac = getCmdLoc c),
+  loads_must_be_in_pre ([ac]++acs) pid (cs3 ++ [c]).
+Proof.
+  intros.
+  apply Forall_forall.
+  intros x Hinx H.
+  destruct_in Hinx.
+    eapply Forall_forall in Hlds; eauto.
+    apply Hlds in H. simpl_env. auto.
+
+    destruct_in Hinx. 
+      destruct ac. simpl in *. subst. auto.
+Qed.
+
+Ltac wf_stld_state_append_tac :=
+  try solve 
+    [apply wf_stld_state_append; simpl; try solve [auto | destruct_dec]].
+
+Lemma find_stld_pair_cmd__wf_stld_state: forall (pid : id) cs c st
+  (Hwfst: wf_stld_state cs pid st),
+  wf_stld_state (cs++[c]) pid (find_stld_pair_cmd pid st c).
+Proof.
+  intros.
+  destruct st as [s acs].
+  destruct c; wf_stld_state_append_tac; simpl.
+    Case "1".        
+      destruct (id_dec pid id5); wf_stld_state_append_tac.
+        subst id5. simpl.
+        exists cs. exists value5. exists align5. exists nil.
+        unfold loads_must_be_in_pre, store_in_cmds. auto.
+    Case "2".
+      destruct value1 as [qid|]; wf_stld_state_append_tac.
+      destruct (id_dec pid qid); wf_stld_state_append_tac.
+        subst qid.
+        destruct s.
+        SCase "2.1".
+          simpl in *. destruct Hwfst.
+          split.
+            apply alloca_in_cmds_merge; auto.
+            apply store_in_cmds_merge; auto.
+        SCase "2.2".
+          simpl in *.
+          destruct Hwfst as [cs3 [ty0 [al0 [cs4 [EQ [Hnst Hnld]]]]]]; subst.
+          exists cs3. exists ty0. exists al0.
+          exists (cs4++[insn_load id5 typ5 (value_id pid) align5]).
+          simpl_env. 
+          split; auto.
+          split.
+            apply store_in_cmds_merge; auto.
+            apply loads_must_be_in_pre_append'; auto.
+              simpl. destruct_dec.
+        SCase "2.3".
+          simpl in *.
+          destruct Hwfst as [cs3 [num0 [al0 [cs4 [EQ [Hnst Hnld]]]]]]; subst.
+          exists cs3. exists num0. exists al0. 
+          exists (cs4++[insn_load id5 typ5 (value_id pid) align5]).
+          simpl_env. 
+          split; auto.
+          split.
+            apply store_in_cmds_merge; auto.
+            apply loads_must_be_in_pre_append'; auto.
+              simpl. destruct_dec.
+    Case "3".
+      destruct value2 as [qid|]; wf_stld_state_append_tac.
+      destruct (id_dec pid qid); wf_stld_state_append_tac.
+        subst qid.
+        destruct s.
+        SCase "3.1".
+          simpl. exists cs. exists typ5. exists align5. exists nil.
+          unfold loads_must_be_in_pre, store_in_cmds. auto.
+        SCase "3.2".
+          simpl in *.
+          destruct Hwfst as [cs3 [ty0 [al0 [cs4 [EQ [Hnst Hnld]]]]]]; subst.
+          exists (cs3 ++ insn_store i0 ty0 v (value_id pid) al0 :: cs4). 
+          exists typ5. exists align5. exists nil.
+          simpl_env. 
+          split; auto.
+          split; auto.
+            constructor.
+        SCase "3.3".
+          simpl in *.
+          destruct Hwfst as [cs3 [num0 [al0 [cs4 [EQ [Hnst Hnld]]]]]]; subst.
+          exists (cs3 ++ insn_alloca pid t num0 al0 :: cs4). 
+          exists typ5. exists align5. exists nil.
+          simpl_env. 
+          split; auto.
+          split; auto.
+            constructor.
+Qed.
+
+Lemma find_stld_pairs_cmds__wf_stld_state_aux: forall (pid : id) cs 
+  cs2 cs1 st1 (Heq: cs = cs1 ++ cs2)
+  (Hwfst: wf_stld_state cs1 pid st1),
+  wf_stld_state cs pid (fold_left (find_stld_pair_cmd pid) cs2 st1).
+Proof.
+  induction cs2 as [|c2 cs2]; simpl; intros; subst; auto.
+    simpl_env. auto.
+
+    apply IHcs2 with (cs3:=cs1++[c2]); simpl_env; auto.
+    clear IHcs2.
+    apply find_stld_pair_cmd__wf_stld_state; auto.
+Qed.
+
+Definition find_stld_pair_cmd' (pid:id) (acc:stld_state * AssocList action) 
+  (c:cmd) : stld_state * option (id * action) :=
+let '(st, actions) := acc in
+match c with
+| insn_alloca qid ty value5 align5 =>
+    if id_dec pid qid
+    then (STLD_alloca ty, None)
+    else (st, None)
+| insn_store sid typ5 v0 value2 align5 =>
+    match value2 with
+    | value_id qid =>
+       if id_dec pid qid
+       then 
+         match st with
+         | STLD_store sid' _ => (STLD_store sid v0, Some (sid', AC_remove))
+         | _ => (STLD_store sid v0, None)
+         end
+      else (st, None)
+    | value_const const5 => (st, None)
+    end
+| insn_load lid typ5 value1 align5 =>
+    match value1 with
+    | value_id qid =>
+       if id_dec pid qid
+       then 
+         match st with
+         | STLD_store _ v' => (st, Some (lid, AC_vsubst v'))
+         | STLD_alloca ty' => (st, Some (lid, AC_tsubst ty'))
+         | _ => (st, None)
+         end
+       else (st, None)
+    | value_const const5 => (st, None)
+    end
+| _ => (st, None)
+end.
+
+Lemma find_stld_pair_cmd__find_stld_pair_cmd': forall pid st1 c,
+  find_stld_pair_cmd pid st1 c =
+  (let (s, o) := find_stld_pair_cmd' pid st1 c in
+   match o with
+   | ret ac => (s, ac :: snd st1)
+   | merror => (s, snd st1)
+   end).
+Proof.
+  destruct st1 as [s1 acc1].
+  destruct c; simpl; intros; auto.
+    destruct_if; uniq_result; auto.
+
+    destruct value1; auto.
+    destruct_if; auto.
+    destruct s1; auto.
+
+    destruct value2; auto.
+    destruct_if; auto.
+    destruct s1; auto.
+Qed.
+
+Lemma find_stld_pairs_cmds__find_stld_pairs_cmds': forall pid cs st1,
+  fold_left (find_stld_pair_cmd pid) cs st1 =
+  fold_left (fun st c => 
+             match find_stld_pair_cmd' pid st c with
+             | (s, Some ac) => (s, ac::snd st)
+             | (s, None) => (s, snd st)
+             end) cs st1.
+Proof.
+  induction cs as [|c cs]; simpl; intros; auto.
+    rewrite IHcs.
+    f_equal.
+    apply find_stld_pair_cmd__find_stld_pair_cmd'.
+Qed.
+
+Lemma find_stld_pair_cmd'__wf_cs_action_pre: forall cs cs1 c cs2 st1 st2 pid 
+  (Heq: cs = cs1 ++ c :: cs2)
+  (Huniq: NoDup (getCmdsLocs cs))
+  (Hwfst1: wf_stld_state cs1 pid st1) ac
+  (Hfind: find_stld_pair_cmd' pid st1 c = (st2, Some ac)),
+  wf_cs_action_pre (snd st1) cs pid ac.
+Proof.
+
+Ltac find_stld_pair_cmd'__wf_cs_action_pre_tac :=
+  match goal with
+  | Huniq: NoDup _ |- context [(?A ++ ?b :: ?C) ++ ?d :: ?E] =>
+    rewrite_env (A++b::(C++d::E));
+    rewrite_env (A++b::(C++d::E)) in Huniq;
+    exists C; exists d; exists E; exists (getCmdsLocs A)
+  end.
+
+  intros. subst.
+  destruct st1 as [s1 acc1]. 
+  destruct c; simpl in Hfind; tinv Hfind.
+  Case "1".
+    destruct_if; tinv Hfind.
+  Case "2".
+    destruct value1; tinv Hfind.
+    destruct_if.
+    destruct s1; inv H0.
+    SCase "2.1".
+      simpl in *.
+      destruct Hwfst1 as [cs3 [ty0 [al0 [cs4 [EQ [Hnst Hnld]]]]]]; subst.
+      exists i0. 
+      find_stld_pair_cmd'__wf_cs_action_pre_tac.
+      split.
+        rewrite getCmdsLocs_app in Huniq. simpl in Huniq.
+        apply find_init_stld_inl_intro; auto.
+      split; auto.
+      split; auto.
+      split; simpl; auto.
+        destruct_dec.
+    SCase "2.2".
+      simpl in *.
+      destruct Hwfst1 as [cs3 [num0 [al0 [cs4 [EQ [Hnst Hnld]]]]]]; subst.
+      find_stld_pair_cmd'__wf_cs_action_pre_tac.
+      split.
+        rewrite getCmdsLocs_app in Huniq. simpl in Huniq.
+        apply find_init_stld_inr_intro; auto.
+      split; auto.
+      split; auto.
+      split; simpl; auto.
+        destruct_dec.
+  Case "3".
+    destruct value2; tinv Hfind.
+    destruct_if.
+    destruct s1; inv H0.
+    simpl in *.
+    destruct Hwfst1 as [cs3 [ty0 [al0 [cs4 [EQ [Hnst Hnld]]]]]]; subst.
+    exists v. 
+    find_stld_pair_cmd'__wf_cs_action_pre_tac.
+    split.
+      rewrite getCmdsLocs_app in Huniq. simpl in Huniq.
+      apply find_init_stld_inl_intro; auto.
+    split; auto.
+    split; simpl; auto.
+      destruct_dec.
+Qed.
+
+Lemma find_stld_pair_cmd__split: forall pid st c st' ac
+  (Hfind: find_stld_pair_cmd pid st c = st') (Hin: In ac (snd st')),
+  In ac (snd st) \/ find_stld_pair_cmd' pid st c = (fst st', Some ac).
+Admitted.
+
+Lemma find_stld_pairs_cmds__split: forall pid s0 acc0 ac cs acs s2
+  (Heq: fold_left (find_stld_pair_cmd pid) cs (s0, acc0) = 
+    (s2, acs ++ acc0))
+  (Hin: In ac acs),
+  exists acs1, exists acs2,
+  exists cs1, exists c, exists cs2, exists s1, exists s,
+    fold_left (find_stld_pair_cmd pid) cs1 (s0, acc0) = (s1, acs1 ++ acc0) /\
+    find_stld_pair_cmd' pid (s1, acs1 ++ acc0) c = (s, Some ac) /\    
+    fold_left (find_stld_pair_cmd pid) cs2 (s, ac::acs1 ++ acc0) = 
+      (s2, acs2 ++ ac :: acs1 ++ acc0).
+Proof.
+  induction cs as [|c cs]; simpl; intros; subst.
+    inversion Heq. admit.
+
+    destruct c; try solve [apply IHcs in Heq; auto].
+Admitted.
+
+End TEST.
+
 (***************************************************************)
 
 Definition wf_cs_action (cs:cmds) (pid:id) (elt:id * action): Prop :=
@@ -2594,15 +3060,6 @@ match ac' with
       Some (inl id') = find_next_stld cs0 pid
 end.
 
-Definition alloca_in_cmd (id':id) (c:cmd) : bool :=
-match c with
-| insn_alloca qid _ _ _ => id_dec id' qid
-| _ => false
-end.
-
-Definition alloca_in_cmds (id':id) (cs:cmds) : bool :=
-(List.fold_left (fun re c => re || alloca_in_cmd id' c) cs false).
-
 Definition wf_stld_state (cs:cmds) (pid:id) (s:stld_state): Prop :=
 match s with
 | STLD_init => alloca_in_cmds pid cs = false /\ store_in_cmds pid cs = false
@@ -2615,17 +3072,6 @@ match s with
       cs = cs1 ++ insn_alloca pid t0 num al :: cs2 /\
       store_in_cmds pid cs2 = false /\ load_in_cmds pid cs2 = false
 end.
-
-Lemma alloca_in_cmds_merge: forall i0 cs1 cs2,
-  alloca_in_cmds i0 cs1 = false /\ alloca_in_cmds i0 cs2 = false ->
-  alloca_in_cmds i0 (cs1++cs2) = false.
-Proof.
-  unfold alloca_in_cmds.
-  intros.
-  rewrite fold_left_app.
-  destruct H as [H1 H2].
-  rewrite H1. auto.
-Qed.
 
 Lemma wf_stld_state_append: forall cs1 pid c s (Hwf: wf_stld_state cs1 pid s)
   (Hnot: alloca_in_cmd pid c = false /\ 
