src3.0/TV/eq_tv_correct.v
@@ -20,7 +20,6 @@ Require Import eq_tv.
 Require Import eq_tv_dec.
 Require Import Coq.Bool.Sumbool.
 Require Import symexe_tactic.
-Require Import sb_metadata.
 
 Ltac repeat_bsplit :=
   repeat (bsplit; auto using eq_sumbool2bool_true).
