src/.dir-locals.el
@@ -5,15 +5,15 @@
 ;; FIXME: maybe we should include just one directory recursively and
 ;; change the Requires correspondingly.
 
-((coq-mode . ((coq-load-path . ("~/src/vol/src/Vellvm"
-                                "~/src/vol/src/Vellvm/ott"
-                                "~/src/vol/src/Vellvm/monads"
-                                "~/src/vol/src/Vellvm/compcert"
-                                "~/src/vol/src/Vellvm/GraphBasics"
-                                "~/src/vol/src/Transforms"
-                                "~/src/vol/src/TV"
-                                "~/src/vol/src/SoftBound"
-                                "~/src/vol/theory/metatheory_8.3"))
+((coq-mode . ((coq-load-path . ("~/SVN/sol/vol/src/Vellvm"
+                                "~/SVN/sol/vol/src/Vellvm/ott"
+                                "~/SVN/sol/vol/src/Vellvm/monads"
+                                "~/SVN/sol/vol/src/Vellvm/compcert"
+                                "~/SVN/sol/vol/src/Vellvm/GraphBasics"
+                                "~/SVN/sol/vol/src/Transforms"
+                                "~/SVN/sol/vol/src/TV"
+                                "~/SVN/sol/vol/src/SoftBound"
+                                "~/SVN/sol/theory/metatheory_8.3"))
               (coq-prog-args . ("-emacs-U" ;; required for Coq to work
                                            ;; with proof general
                                 "-impredicative-set")))))
